coq-SystemRF-3.0/Denotations/BasicPropsDenotes.v
@@ -258,18 +258,31 @@ Proof. intros a t_a t v v' k.
   apply lem_denotes_tsubFTV_self' with (depth t); trivial. Qed.
 
 
+Lemma lem_erase_self_tsubFTV :
+  forall (a:vname) (t_a t:type) (v:expr) (k :kind),
+    noExists t_a -> erase (self (tsubFTV a t_a t) (subFTV a t_a v) k) 
+                      = erase (tsubFTV a t_a (self t v k)).
+Proof. intros a t_a; induction t; intros v k' H;
+  destruct k'; repeat rewrite lem_self_star; trivial;
+  try destruct b eqn:B; simpl;
+  try destruct (a =? a0) eqn:A; simpl; try reflexivity.
+  - (* TRefn Base *) destruct t_a; simpl in H; simpl;
+    try contradiction; reflexivity.
+  - (* TExists Base *) apply IHt2; apply H.
+  Qed.
+
 Lemma lem_denotes_self_tsubFTV' : 
   forall (n:nat) (a:vname) (t_a t:type) (v v':expr) (k:kind),
-    depth t <= n -> noExists t_a -> isLCT t_a -> freeTV t_a = empty
-        -> subFTV a t_a v = v -> isLC v
+    depth t <= n -> noExists t_a 
+        -> isLCT t_a -> freeTV t_a = empty -> isLC v
         -> Denotes (tsubFTV a t_a (self t v k)) v'
-        -> Denotes (self (tsubFTV a t_a t)  v  k) v'.
+        -> Denotes (self (tsubFTV a t_a t) (subFTV a t_a v)  k) v'.
 Proof. induction n.
-  - (* n = 0 => TRefn *) intros; revert H5;
+  - (* n = 0 => TRefn *) intros; revert H4;
     assert (depth t = 0) by auto with *;
-    destruct t; simpl in H5; try discriminate;
+    destruct t; simpl in H4; try discriminate;
     destruct k; try repeat rewrite lem_self_star; trivial. 
-    destruct b; simpl; rewrite H3;
+    destruct b; simpl; 
     unfold eqlPred; trivial. (* FTV a0 remains*)
     destruct (a =? a0) eqn:A; simpl; 
     unfold eqlPred; trivial.
@@ -277,42 +290,45 @@ Proof. induction n.
     simpl; trivial; unfold eqlPred.
     repeat rewrite Denotes_equation_1; intuition.
     apply PECons; fold subBV_at; fold psubBV_at;
-    inversion H9; try apply H12. 
+    inversion H8; try apply H11. 
     destruct (0 =? 0) eqn:Z; simpl in Z; try discriminate;
     destruct b eqn:B; unfold isLCT in H1; simpl in H2;
     try destruct i; try destruct H1; try inversion H1;
     try apply (empty_no_elem (names_add a1 (ftvP ps0))) with a1 in H2;
     try apply not_elem_names_add_elim in H2; try destruct H2; intuition.
     * (* TBool *) 
-      apply AddStep with (App (App (Prim Eqv) (subBV_at 0 v' v)) v').
+      set (w := subBV_at 0 v' (subFTV a (TRefn TBool ps0) v)) in *.
+      apply AddStep with (App (App (Prim Eqv) w) v').
       apply EApp1; apply EApp1; apply lem_step_eql_tbool.
       apply lem_decompose_evals with 
-        (App (App (AppT (Prim Eql) (TRefn TBool (psubBV_at 1 v' ps0))) (subBV_at 0 v' v)) v');
+        (App (App (AppT (Prim Eql) (TRefn TBool (psubBV_at 1 v' ps0))) w) v');
       trivial; try apply val_Bc; apply lem_step_evals;
       apply EApp1; apply EApp1; apply lem_step_eql_tbool.
     * (* TInt *) 
-      apply AddStep with (App (App (Prim Eq) (subBV_at 0 v' v)) v').
+      set (w := subBV_at 0 v' (subFTV a (TRefn TInt ps0) v)) in *.
+      apply AddStep with (App (App (Prim Eq) w) v').
       apply EApp1; apply EApp1; apply lem_step_eql_tint.
       apply lem_decompose_evals with 
-        (App (App (AppT (Prim Eql) (TRefn TInt (psubBV_at 1 v' ps0))) (subBV_at 0 v' v)) v');
+        (App (App (AppT (Prim Eql) (TRefn TInt (psubBV_at 1 v' ps0))) w) v');
       trivial; try constructor; apply lem_step_evals;
       apply EApp1; apply EApp1; apply lem_step_eql_tint.
   - (* n > 0 *) intros; destruct t.
-    * (* TRefn *) apply IHn; revert H5; simpl; auto with *.
-    * (* TFunc *) destruct k; simpl; simpl in H5; apply H5.
-    * (* TExists *) revert H5; destruct k; simpl; trivial.
+    * (* TRefn *) apply IHn; revert H4; simpl; auto with *.
+    * (* TFunc *) destruct k; simpl; simpl in H4; apply H4.
+    * (* TExists *) revert H4; destruct k; simpl; trivial.
       (* Base *) repeat rewrite Denotes_equation_3;
-      simpl; rewrite lem_erase_tsubFTV_self; intuition;
-      destruct H8 as [v_x H8]; exists v_x; intuition.
-      rewrite lem_tsubBV_self; trivial.
-      apply lem_den_hasftype in H8 as H9.
-      apply lem_fv_subset_bindsF in H9 as H9;
-      destruct H9; unfold Subset in H11; simpl in H11;
+      simpl. rewrite lem_erase_self_tsubFTV; intuition;
+      destruct H7 as [v_x H7]; exists v_x; intuition.
+      rewrite lem_tsubBV_self; 
+      try apply lem_islc_at_subFTV; trivial.
+      apply lem_den_hasftype in H7 as H8.
+      apply lem_fv_subset_bindsF in H8 as H8;
+      destruct H8; unfold Subset in H10; simpl in H10;
       assert (subFTV a t_a v_x = v_x)
-        by (apply lem_subFTV_notin; unfold not; apply H11). 
-      trivial || rewrite <- H12; rewrite <- H12 in H10.
+        by (apply lem_subFTV_notin; unfold not; apply H10). 
+      trivial || rewrite <- H11; rewrite <- H11 in H9.
       rewrite <- lem_commute_tsubFTV_tsubBV;
-      try rewrite <- lem_commute_tsubFTV_tsubBV in H10;
+      try rewrite <- lem_commute_tsubFTV_tsubBV in H9;
       try assumption.
       try apply IHn; simpl in H; apply Nat.succ_le_mono in H;
       try rewrite <- lem_tsubBV_self;
@@ -320,16 +336,15 @@ Proof. induction n.
       try apply Nat.le_trans with (max (depth t1) (depth t2));
       try apply Nat.le_max_r;
       unfold isLC; simpl; trivial.
-    * (* TPoly *) destruct k; simpl; simpl in H5; apply H5.
-    * (* TList *) destruct k; simpl; simpl in H5; apply H5.
+    * (* TPoly *) destruct k; simpl; simpl in H4; apply H4.
+    * (* TList *) destruct k; simpl; simpl in H4; apply H4.
   Qed.
   
 Lemma lem_denotes_self_tsubFTV : 
   forall (a:vname) (t_a t:type) (v v':expr) (k:kind),
-    noExists t_a -> isLCT t_a -> freeTV t_a = empty
-        -> subFTV a t_a v = v -> isLC v
+    noExists t_a -> isLCT t_a -> freeTV t_a = empty -> isLC v
         -> Denotes (tsubFTV a t_a (self t v k)) v'
-        -> Denotes (self (tsubFTV a t_a t) v k) v'.
+        -> Denotes (self (tsubFTV a t_a t) (subFTV a t_a v) k) v'.
 Proof. intros a t_a t v v' k.
   apply lem_denotes_self_tsubFTV' with (depth t); trivial. Qed.
 
@@ -401,11 +416,6 @@ Proof. induction th; intros t v v' k H1 H2 H3 H4 H5; trivial;
   destruct H1; destruct H0; destruct H2; destruct H3; destruct H4.
   - (* CCons *) simpl; rewrite lem_tsubFV_self; apply IHth;
     try apply lem_islc_at_subFV; auto with *.
-    (*assert (Subset (ftv (subFV x v_x v)) (union (ftv v) (ftv v_x)))
-      by apply ftv_subFV_elim;
-    rewrite H0 in H10; rewrite H6 in H10;
-    apply no_elem_empty; unfold not; intros;
-    apply H10 in H11; intuition. *)
   - (* CConsT *) intros;  
     pose proof (matchesExFTV_dec a t) as Hm; destruct Hm.
     * (* Yes *) destruct t eqn:T; try destruct b; remember H10 as H11;
@@ -416,33 +426,38 @@ Proof. induction th; intros t v v' k H1 H2 H3 H4 H5; trivial;
         rewrite lem_ctsubst_self_FTV with th a (TRefn (FTV a) ps) v k in H9;
         try apply lem_denotes_self_tsubFTV in H9;
         try apply lem_subFTV_notin;
-        try apply lem_csubst_isLC.
-        assert (ftv (csubst th v) = empty)
-          by (apply lem_csubst_pres_noftv; trivial);
-        try rewrite H12; auto.
-        assert (subFTV a t_a v = v)
-          by (apply lem_subFTV_notin; rewrite H6; auto);
-          rewrite <- H14 in H10.
-        rewrite <- lem_unroll_ctsubst_tv_left in H10;
+        try apply lem_csubst_isLC; auto.
+        rewrite <- lem_unroll_ctsubst_tv_left in H9;
+        try rewrite <- lem_unroll_csubst_tv_left in H9;
         try apply H10; intuition.
-      + rewrite lem_unroll_ctsubst_tv_left in H10;
-        try split; destruct H8; trivial;
-        rewrite lem_ctsubst_self_FTV with th a (TExists t0_1 t0_2) v k in H10;
-        try apply lem_denotes_self_tsubFTV in H10;
+      + rewrite lem_unroll_ctsubst_tv_left in H9;
+        try split; destruct H7; trivial;
+        rewrite lem_ctsubst_self_FTV with th a (TExists t0_1 t0_2) v k in H9;
+        try apply lem_denotes_self_tsubFTV in H9;
         try apply lem_subFTV_notin;
         try apply lem_csubst_isLC;
-        assert (ftv (csubst th v) = empty)
-          by (apply lem_csubst_pres_noftv; trivial);
-        try rewrite H14;  
-        assert (subFTV a t_a v = v)
-          by (apply lem_subFTV_notin; rewrite H6; auto);
-        try rewrite <- H15 in H10; 
-        try rewrite <- lem_unroll_ctsubst_tv_left in H10;
-        try apply H10; simpl; auto.
-    * (* No *) simpl; 
-      try apply IHth; try rewrite <- lem_tsubFTV_self_noFTV;
-      simpl in H10; destruct H8;
-      assert (subFTV a t_a v = v)
-          by (apply lem_subFTV_notin; rewrite H6; auto);
-      try apply H10; try rewrite H13; trivial.
+        try rewrite <- lem_unroll_ctsubst_tv_left in H9;
+        try rewrite <- lem_unroll_csubst_tv_left in H9;
+        try apply H9; simpl; auto.
+    * (* No *) simpl; try apply IHth; 
+      try rewrite <- lem_tsubFTV_self_noFTV;
+      simpl in H9; destruct H7;
+      try apply lem_islc_at_subFTV; trivial.
   Qed.  
+
+
+Lemma lem_denotes_eqlLen_ctsubst : 
+  forall (th:csub) (t:type) (v v':expr) (ps:preds),
+    closed th -> loc_closed th -> substitutable th -> uniqueC th 
+        -> isLC v (*-> ftv v = empty*)
+        -> Denotes (ctsubst th (TList t (PCons (eqlLenPred t v) ps))) v'
+        -> Denotes (TList (ctsubst th t) 
+                      (PCons (eqlLenPred (ctsubst th t) (csubst th v)) 
+                                (cpsubst th ps))) v'.
+Proof. intros th t v v' ps H1 H2 H3 H4 H5;
+  unfold eqlLenPred; unfold eq; unfold length;
+  rewrite lem_ctsubst_list; rewrite lem_cpsubst_pcons;
+  repeat rewrite lem_csubst_app;
+  rewrite lem_csubst_prim; rewrite lem_csubst_appT;
+  rewrite lem_csubst_prim; rewrite lem_csubst_bv; trivial.
+Qed.
