coq-SystemRF-3.0/Denotations/SelfifyDenotations.v
@@ -14,9 +14,11 @@ Require Import SystemRF.LemmasTransitive.
 Require Import Denotations.ClosingSubstitutions.
 Require Import Denotations.Denotations.
 Require Import Denotations.BasicPropsCSubst.
+Require Import Denotations.BasicPropsSemantics.
 Require Import Denotations.PrimitivesSemantics.
 Require Import Denotations.PrimitivesDenotations.
 
+Require Import Arith.
 Require Import ZArith.
 
 Lemma lem_denotations_selfify' : forall (n:nat) (g:env) (t:type) (k:kind) (v:expr),
@@ -177,3 +179,384 @@ Proof. intros. apply lemma_list_values with v (erase t) in H1 as vlis;
     try exists n; try split; try subst n';
     try apply val_Bc; try subst p; trivial.
   Qed.
+
+Lemma lem_free_safeListVarUseT : forall (x:vname) (t:type),
+    free t = empty -> safeListVarUseT x t.
+Proof. induction t; simpl; intros; try split;
+  try apply IHt1; try apply IHt2; try apply IHt;
+  try apply no_elem_empty; intros;
+  try apply empty_no_elem with (fvP ps) x in H;
+  try apply empty_no_elem with (union (free t1) (free t2)) x0 in H;
+  try apply empty_no_elem with (union (free t) (fvP ps)) x0 in H;
+  try apply empty_no_elem with (union (free t) (fvP ps)) x in H;
+  try apply empty_no_elem with (free t) x0 in H;
+  try apply not_elem_union_elim in H; try apply H;
+  try destruct H; trivial. 
+Qed.
+
+Lemma lem_free_safeListVarUseE : forall (x:vname) (e:expr),
+    fv e = empty -> safeListVarUseE x e.
+Proof. induction e; simpl; intros; try discriminate;
+  try right; try right;
+  try split; try split; try (apply empty_no_elem; apply H);
+  try apply IHe; try apply IHe1; try apply IHe2; try apply IHe3;
+  try apply lem_free_safeListVarUseT; try apply no_elem_empty; intros;
+  try apply empty_no_elem with (union (fv e1) (fv e2)) x0 in H;
+  try apply empty_no_elem with (union (fv e1) (fv e2)) x  in H;
+  try apply empty_no_elem with (union (fv e) (free t)) x0 in H;
+  try apply empty_no_elem 
+    with (union (fv e1) (union (fv e2) (fv e3))) x0 in H;
+  try apply not_elem_union_elim in H;  try destruct H; 
+  try apply not_elem_union_elim in H0; trivial;
+  try destruct H0; trivial.
+Qed.
+
+Lemma lem_fvP_safeListVarUseP : forall (x:vname) (ps:preds),
+    fvP ps = empty -> safeListVarUseP x ps.
+Proof. induction ps; simpl; intros; trivial; split;
+  try apply IHps; try apply lem_free_safeListVarUseE; 
+  try apply no_elem_empty; intros;
+  try apply empty_no_elem with (union (fv p) (fvP ps)) x0 in H;
+  try apply not_elem_union_elim in H;  try destruct H; trivial.
+Qed.
+
+Lemma lem_safeListVarUseP_strength : forall (x:vname) (ps qs:preds),
+    safeListVarUseP x ps -> safeListVarUseP x qs 
+        -> safeListVarUseP x (strengthen ps qs).
+Proof. intro x; induction ps; simpl; intros; try split;
+  try destruct H; try apply IHps; trivial. Qed.
+
+Lemma lem_safeListVarUseT_push : forall (t:type) (ps:preds) (x:vname),
+    free t = empty -> noExists t -> ~ Elem x (fvP ps)
+        -> safeListVarUseT x (push ps t).
+Proof. induction t; simpl; intros.
+  - apply not_elem_subset with (union (fvP ps0) (fvP ps));
+    try apply fv_strengthen_elim; apply not_elem_union_intro;
+    try apply H1; try apply empty_no_elem; apply H.
+  - split; apply lem_free_safeListVarUseT; try apply no_elem_empty;
+    intros; apply empty_no_elem with (union (free t1) (free t2)) x0 in H;
+    try apply not_elem_union_elim in H; try destruct H; trivial.
+  - contradiction.
+  - apply lem_free_safeListVarUseT; apply H.
+  - split; try apply lem_free_safeListVarUseT; try apply no_elem_empty;
+    intros; apply empty_no_elem with (union (free t) (fvP ps)) x in H as H';
+    try apply empty_no_elem with (union (free t) (fvP ps)) x0 in H;
+    try apply not_elem_union_elim in H'; try destruct H'; 
+    try apply not_elem_union_elim in H;  try destruct H; trivial.
+Qed.
+
+
+Lemma lem_safeListVarUseT_tsubFV : forall (t:type) (x:vname) (v:expr),
+    safeListVarUseT x t -> tsubFV x v t = t.
+Proof. induction t; simpl; intros.
+  - rewrite lem_psubFV_notin; trivial.
+  - destruct H; rewrite IHt1; try rewrite IHt2; trivial.
+  - destruct H; rewrite IHt1; try rewrite IHt2; trivial.
+  - rewrite IHt; trivial.
+  - rewrite IHt; try rewrite lem_psubFV_notin; destruct H; trivial.
+Qed.
+
+Lemma lem_safeListVarUseT_ctsubst : forall (t:type) (x:vname) (th:csub),
+    closed th -> substitutable th -> uniqueC th
+      -> safeListVarUseT x t -> safeListVarUseT x (ctsubst th t).
+Proof. induction t; simpl; intros.
+  - destruct b eqn:B.
+    * rewrite lem_ctsubst_refn; try left; simpl;
+      try apply not_elem_subset with (fvP ps);
+      try apply lem_fvP_cpsubst; trivial.
+    * rewrite lem_ctsubst_refn; try left; simpl;
+      try apply not_elem_subset with (fvP ps);
+      try apply lem_fvP_cpsubst; trivial.
+    * rewrite lem_ctsubst_refn; try right; simpl;
+      try apply not_elem_subset with (fvP ps);
+      try apply lem_fvP_cpsubst; trivial.
+    * simpl; destruct (elem_dec a (tvbindsC th)).
+      + apply lem_tvbindsC_tvboundinC in H3;
+        destruct H3 as [t_a H3].
+        rewrite lem_ctsubst_refn_tv with th a t_a ps;
+        try apply lem_safeListVarUseT_push;
+        try apply lem_tvboundinC_closed with a th;
+        try apply lem_tvboundinC_substitutable with a th;
+        try apply not_elem_subset with (fvP ps);
+        try apply lem_fvP_cpsubst; trivial.
+      + rewrite lem_ctsubst_refn_tv_notin'; simpl; try apply H3;
+        try apply not_elem_subset with (fvP ps);
+        try apply lem_fvP_cpsubst; trivial.
+  - rewrite lem_ctsubst_func; simpl; split; apply IHt1 || apply IHt2;
+    destruct H2; trivial.
+  - rewrite lem_ctsubst_exis; simpl; split; apply IHt1 || apply IHt2;
+    destruct H2; trivial.
+  - rewrite lem_ctsubst_poly; simpl; apply IHt; trivial.
+  - rewrite lem_ctsubst_list; simpl; split; try apply IHt;
+    destruct H2; try apply not_elem_subset with (fvP ps);
+    try apply lem_fvP_cpsubst; trivial.
+Qed.
+  
+Lemma lem_safeListVarUseE_csubst : forall (e:expr) (x:vname) (th:csub),
+    closed th -> substitutable th -> uniqueC th -> ~ in_csubst x th
+      -> safeListVarUseE x e -> safeListVarUseE x (csubst th e).
+Proof. induction e; simpl; intros; try contradiction.
+  - rewrite lem_csubst_bc; simpl; exact I.
+  - rewrite lem_csubst_ic; simpl; exact I.
+  - rewrite lem_csubst_prim; simpl; exact I.
+  - rewrite lem_csubst_bv; simpl; exact I.
+  - destruct (elem_dec x (vbindsC th)).
+    * apply lem_vbindsC_boundinC in H4; destruct H4 as [v_x H4]. 
+      apply lem_csubst_fv_boundinC in H4 as H5; try rewrite H5;
+      try apply lem_free_safeListVarUseE;
+      try apply lem_boundinC_closed in H4; try destruct H4;
+      simpl; trivial.
+    * rewrite lem_csubst_fv'; simpl; trivial.
+  - rewrite lem_csubst_lambda; simpl;
+    apply not_elem_subset with (fv e); try apply lem_fv_csubst; trivial.
+  - rewrite lem_csubst_app; simpl; destruct H3; try destruct H3.
+    * left; split; destruct e1; simpl in H3; try contradiction;
+      subst e1 e2; try rewrite lem_csubst_appT;
+      try rewrite lem_csubst_prim; try rewrite lem_csubst_fv; 
+      simpl; trivial.
+    * right; left; split; destruct H3;
+      destruct e1; simpl in H3; try contradiction;
+      subst e1; try rewrite lem_csubst_appT;
+      try rewrite lem_csubst_prim; try apply IHe2; simpl; trivial.
+    * right; right; split; destruct H3; try apply IHe1;
+      try apply IHe2; trivial.
+  - rewrite lem_csubst_lambdaT; simpl;
+    apply not_elem_subset with (fv e); try apply lem_fv_csubst; trivial.
+  - rewrite lem_csubst_appT; simpl; split; destruct H3;
+    try apply IHe; try apply lem_safeListVarUseT_ctsubst; trivial.
+  - rewrite lem_csubst_let; simpl; split; destruct H3;
+    try apply IHe1; try apply H2;
+    try apply not_elem_subset with (fv e2); try apply lem_fv_csubst; trivial.
+  - rewrite lem_csubst_annot; simpl; split; destruct H3;
+    try apply IHe; try apply lem_safeListVarUseT_ctsubst; trivial.
+  - rewrite lem_csubst_if; simpl; repeat split; destruct H3;
+    destruct H4; try apply IHe1; try apply IHe2; try apply IHe3; trivial.
+  - rewrite lem_csubst_nil; trivial.
+  - rewrite lem_csubst_cons; simpl; split; destruct H3;
+    try apply IHe1; try apply IHe2; trivial.
+  - rewrite lem_csubst_switch; simpl; repeat split; destruct H3;
+    destruct H4; try apply IHe1; try apply IHe2; try apply IHe3; trivial.
+  - rewrite lem_csubst_error; trivial.
+Qed.
+  
+Lemma lem_safeListVarUseP_csubst : forall (ps:preds) (x:vname) (th:csub),
+    closed th -> substitutable th -> uniqueC th -> ~ in_csubst x th
+      -> safeListVarUseP x ps -> safeListVarUseP x (cpsubst th ps).
+Proof. induction ps; simpl; intros.
+  - rewrite lem_cpsubst_pempty; trivial.
+  - rewrite lem_cpsubst_pcons; simpl; split; destruct H3;
+    try apply lem_safeListVarUseE_csubst; try apply IHps; trivial.
+Qed.
+
+
+Lemma lem_safeListVarUseE_eqlLen' : 
+  forall (x:vname) (e:expr) (t:type) (v v' vf:expr) (m:Z),
+    safeListVarUseE x e -> isValue v -> isValue v' -> isValue vf
+      -> EvalsTo (length t v) (Ic m) -> EvalsTo (length t v') (Ic m)
+      -> EvalsTo (subFV x v  e) vf
+      -> EvalsTo (subFV x v' e) vf.
+Proof. intro x; induction e; intros; simpl in H;
+  try contradiction; simpl in *; trivial.
+  - (* FV *) apply Nat.eqb_neq in H; rewrite H in *; trivial.
+  - (* Lambda *) rewrite lem_subFV_notin' in H5;
+    try rewrite lem_subFV_notin'; trivial.
+  - (* App *) repeat destruct H.
+    (* length call *) destruct e1; simpl in H; try contradiction;
+    subst e1 e2; simpl in H5; simpl;
+    assert (x =? x = true) as X by (apply Nat.eqb_eq; reflexivity);
+    rewrite X in *;   
+    inversion H3; inversion H;
+    try ( apply lem_value_stuck in H13; trivial; contradiction );
+    try ( inversion H12; try inversion pf; 
+          apply lem_value_stuck in H17; try apply val_Prm; contradiction ).
+    inversion H4; inversion H14;
+    try ( apply lem_value_stuck in H21; try apply val_Len; contradiction );
+    try ( apply lem_value_stuck in H22; trivial; contradiction ).
+    inversion H5; try (rewrite <- H24 in H2; inversion H2);
+    inversion H23;
+    try ( apply lem_value_stuck in H30; try apply val_Len; contradiction );
+    try ( apply lem_value_stuck in H31; trivial; contradiction ).
+    rewrite deltaM_pf_indep with Length v pf1 pf in H28; subst e2 e7.
+    assert (vf = (Ic m))
+      by (apply lem_evals_val_det with (deltaM Length v pf);
+          try apply val_Ic; trivial); subst vf e8;
+    apply AddStep with e4; subst e4; try apply EPrimM; trivial.
+    
+    (* length call not x*) destruct e1; simpl in H; try contradiction.
+    subst e1; simpl in H5; simpl. 
+    apply lem_app_evals_val in H5 as Happ;
+    try destruct Happ as [_ [v2 [_ [val2 [_ ev_e2v_v2]]]]]; try apply H2.
+    apply IHe2 with t v v' v2 m in ev_e2v_v2 as ev_e2v'_v2; trivial.
+    assert (EvalsTo (App (AppT (Prim Length) (tsubFV x v t0)) 
+                         (subFV x v e2)) 
+                    (App (AppT (Prim Length) (tsubFV x v t0)) v2))
+      by (apply lemma_app_many2; try apply val_Len; trivial).
+    apply lemma_evals_trans 
+      with (App (AppT (Prim Length) (tsubFV x v' t0)) v2); 
+    try apply lemma_app_many2; try apply val_Len; trivial.
+    apply lem_decompose_evals 
+      with (App (AppT (Prim Length) (tsubFV x v t0)) (subFV x v e2))
+           (App (AppT (Prim Length) (tsubFV x v t0)) v2) vf in H5; 
+    trivial. inversion H5; try (rewrite <- H8 in H2; inversion H2).
+    inversion H7;
+    try ( apply lem_value_stuck in H14; try apply val_Len; contradiction );
+    try ( apply lem_value_stuck in H15; trivial; contradiction ).
+    apply AddStep with e0; subst e0; try apply EPrimM; trivial.    
+    
+    (* otherwise *) apply lem_app_evals_val in H5 as Happ;
+    try destruct Happ as [v1 [v2 [val1 [val2 [ev_e1v_v1 ev_e2v_v2]]]]];
+    try apply H2;
+    apply IHe1 with t v v' v1 m in ev_e1v_v1 as ev_e1v'_v1; 
+    try apply IHe2 with t v v' v2 m in ev_e2v_v2 as ev_e2v'_v2;
+    trivial; assert (EvalsTo (App (subFV x v e1) (subFV x v e2)) (App v1 v2))
+      by (apply lemma_app_both_many; trivial);
+    apply lemma_evals_trans with (App v1 v2);
+    try apply lemma_app_both_many; trivial;
+    apply lem_decompose_evals with (App (subFV x v e1) (subFV x v e2)); trivial.
+  - (* LambdaT *) rewrite lem_subFV_notin' in H5;
+    try rewrite lem_subFV_notin'; trivial.
+  - (* AppT *) destruct H;
+    rewrite lem_safeListVarUseT_tsubFV in H5;
+    try rewrite lem_safeListVarUseT_tsubFV;
+    try apply lem_appT_evals_val in H5 as HappT;
+    try destruct HappT as [v1 [val1 ev_ev_v1]];
+    try apply IHe with t0 v v' v1 m in ev_ev_v1 as ev_ev'_v1; trivial.
+    inversion H5.
+    * subst vf; inversion H2; destruct e; simpl in H; try contradiction;
+      simpl in H9; try discriminate; simpl; rewrite H9; try apply Refl.
+      apply Nat.eqb_neq in H; rewrite H; apply Refl.
+    * inversion H7;
+      assert (EvalsTo (AppT (subFV x v e) t) (AppT v1 t))
+        by (apply lemma_appT_many; trivial);
+      apply lemma_evals_trans with (AppT v1 t);
+      try apply lemma_appT_many; trivial;
+      apply lem_decompose_evals with (AppT (subFV x v e) t); trivial.
+  - (* Let *) destruct H; rewrite (lem_subFV_notin' e2) in H5;
+    try rewrite (lem_subFV_notin' e2); trivial;
+    apply lem_let_evals_val in H5 as Hlet; try apply H2;
+    try destruct Hlet as [v1 [val1 [ev_e1v_v1 ev_e2v1_vf]]].
+    apply IHe1 with t v v' v1 m in ev_e1v_v1 as ev_e1v'_v1; trivial.
+    try apply lemma_evals_trans with (Let v1 e2);
+    try apply lemma_let_many; try apply ev_e1v'_v1;
+    apply AddStep with (subBV v1 e2); try apply ELetV; trivial.
+  - (* Annot *) destruct H;
+    rewrite lem_safeListVarUseT_tsubFV in H5;
+    try rewrite lem_safeListVarUseT_tsubFV;
+    try apply lem_ann_evals_val in H5 as Hann;
+    try destruct Hann as [v1 [val1 ev_ev_v1]];
+    try apply IHe with t0 v v' v1 m in ev_ev_v1 as ev_ev'_v1; trivial.
+    assert (EvalsTo (Annot (subFV x v e) t) (Annot v1 t))
+      by (apply lemma_annot_many; trivial).
+    apply lemma_evals_trans with (Annot v1 t);
+    try apply lemma_annot_many; trivial;
+    apply lem_decompose_evals with (Annot (subFV x v e) t); trivial.
+  - (* If *) destruct H; destruct H6;
+    try apply lem_if_evals_val in H5 as Hif; try apply H2;
+    destruct Hif as [v'' [val' Hif]]; destruct Hif; destruct H8.
+    * apply IHe1 with t v v' (Bc true) m in H8 as ev_e1v'_tt; 
+      try apply val_Bc; trivial.
+      assert (EvalsTo (If (subFV x v e1) (subFV x v e2) (subFV x v e3)) 
+                      (If (Bc true) (subFV x v e2) (subFV x v e3)))
+        by (apply lemma_if_many; trivial).
+      apply lemma_evals_trans 
+        with (If (Bc true) (subFV x v' e2) (subFV x v' e3));
+      try apply lemma_if_many; trivial.
+      assert (EvalsTo (If (Bc true) (subFV x v e2) (subFV x v e3)) vf)
+        by (apply lem_decompose_evals 
+              with (If (subFV x v e1) (subFV x v e2) (subFV x v e3)); trivial).
+      inversion H11; try (subst vf; inversion H2; contradiction);
+      inversion H12; 
+      try (apply lem_value_stuck in H20; try apply val_Bc; contradiction).
+      subst e4; apply AddStep with (subFV x v' e2);
+      try apply EIfT; apply IHe2 with t v m; trivial.
+    * apply IHe1 with t v v' (Bc false) m in H8 as ev_e1v'_tt; 
+      try apply val_Bc; trivial.
+      assert (EvalsTo (If (subFV x v e1) (subFV x v e2) (subFV x v e3)) 
+                      (If (Bc false) (subFV x v e2) (subFV x v e3)))
+        by (apply lemma_if_many; trivial).
+      apply lemma_evals_trans 
+        with (If (Bc false) (subFV x v' e2) (subFV x v' e3));
+      try apply lemma_if_many; trivial.
+      assert (EvalsTo (If (Bc false) (subFV x v e2) (subFV x v e3)) vf)
+        by (apply lem_decompose_evals 
+              with (If (subFV x v e1) (subFV x v e2) (subFV x v e3)); trivial).
+      inversion H11; try (subst vf; inversion H2; contradiction);
+      inversion H12; 
+      try (apply lem_value_stuck in H20; try apply val_Bc; contradiction).
+      subst e4; apply AddStep with (subFV x v' e3);
+      try apply EIfF; apply IHe3 with t v m; trivial.
+  - (* Cons *) destruct H; apply lem_cons_evals_val in H5 as Happ;
+    try destruct Happ as [v1 [v2 [val1 [val2 [ev_e1v_v1 ev_e2v_v2]]]]];
+    try apply H2;
+    apply IHe1 with t v v' v1 m in ev_e1v_v1 as ev_e1v'_v1; 
+    try apply IHe2 with t v v' v2 m in ev_e2v_v2 as ev_e2v'_v2;
+    trivial; assert (EvalsTo (Cons (subFV x v e1) (subFV x v e2)) (Cons v1 v2))
+      by (apply lemma_cons_both_many; trivial);
+    apply lemma_evals_trans with (Cons v1 v2);
+    try apply lemma_cons_both_many; trivial;
+    apply lem_decompose_evals with (Cons (subFV x v e1) (subFV x v e2)); trivial.
+  - (* Switch *) destruct H; destruct H6;
+    try apply lem_switch_evals_val in H5 as Hsw; try apply H2;
+    destruct Hsw as [v'' [val' Hsw]]; destruct Hsw. 
+    * destruct H8; apply IHe1 with t v v' Nil m in H8 as ev_e1v'_nl; 
+      try apply val_Nil; trivial.
+      assert (EvalsTo (Switch (subFV x v e1) (subFV x v e2) (subFV x v e3)) 
+                      (Switch Nil (subFV x v e2) (subFV x v e3)))
+        by (apply lemma_switch_many; trivial).
+      apply lemma_evals_trans 
+        with (Switch Nil (subFV x v' e2) (subFV x v' e3));
+      try apply lemma_switch_many; trivial.
+      assert (EvalsTo (Switch Nil  (subFV x v e2) (subFV x v e3)) vf)
+        by (apply lem_decompose_evals 
+              with (Switch (subFV x v e1) (subFV x v e2) (subFV x v e3)); trivial).
+      inversion H11; try (subst vf; inversion H2; contradiction);
+      inversion H12;
+      try (apply lem_value_stuck in H20; try apply val_Nil; contradiction).
+      subst e4; apply AddStep with (subFV x v' e2);
+      try apply ESwitchN; apply IHe2 with t v m; trivial.
+    * destruct H8 as [v1 [v2 [val1 [val2 [ev_e1v_cn ev_e3v_v'']]]]];
+      apply IHe1 with t v v' (Cons v1 v2) m in ev_e1v_cn as ev_e1v'_cn; 
+      try apply val_Cons; trivial.
+      assert (EvalsTo (Switch (subFV x v e1) (subFV x v e2) (subFV x v e3)) 
+                      (Switch (Cons v1 v2) (subFV x v e2) (subFV x v e3)))
+        by (apply lemma_switch_many; trivial).
+      apply lemma_evals_trans 
+        with (Switch (Cons v1 v2) (subFV x v' e2) (subFV x v' e3));
+      try apply lemma_switch_many; trivial.
+      assert (EvalsTo (Switch (Cons v1 v2)  (subFV x v e2) (subFV x v e3)) vf)
+        by (apply lem_decompose_evals 
+              with (Switch (subFV x v e1) (subFV x v e2) (subFV x v e3)); trivial).
+      inversion H9; try (subst vf; inversion H2; contradiction);
+      inversion H10;
+      try ( apply lem_value_stuck in H18; try apply val_Cons; 
+            trivial; contradiction ).
+      subst e4; apply AddStep with (App (App (subFV x v' e3) v1) v2);
+      try apply ESwitchC; try apply IHe3 with t v m; trivial.
+      apply lem_app_evals_val in H11; try apply H2;
+      destruct H11 as [v3' [_ [val3' [_ [ev_e3v'_v3' _]]]]];
+      apply lem_app_evals_val in ev_e3v'_v3'; try apply val3';
+      destruct ev_e3v'_v3' as [v3'' [_ [val3'' [_ [ev_e3v_v3'' _]]]]];
+      apply IHe3 with t v v' v3'' m in ev_e3v_v3'' as ev_e3v'_v3'';
+      trivial; apply lemma_evals_trans with (App (App v3'' v1) v2);
+      try apply lemma_app_many; try apply lemma_app_many; trivial.
+      inversion H9; try (subst vf e5; inversion H2; contradiction).
+      inversion H11;
+      try ( apply lem_value_stuck in H27; try apply val_Cons; 
+            trivial; contradiction ).
+      subst e6; apply lem_decompose_evals 
+        with (App (App (subFV x v e3) v1) v2); 
+      try apply lemma_app_many; try apply lemma_app_many; trivial.
+Qed.
+
+Lemma lem_safeListVarUseP_eqlLen : 
+  forall (x:vname) (ps:preds) (t:type) (v v':expr) (m:Z),
+    safeListVarUseP x ps -> isValue v -> isValue v'
+      -> EvalsTo (length t v) (Ic m) -> EvalsTo (length t v') (Ic m)
+      -> PEvalsTrue (psubFV x v ps) -> PEvalsTrue (psubFV x v' ps).
+Proof. intro x; induction ps; simpl; intros; trivial.
+  try apply PECons; inversion H4; destruct H.
+  - apply lem_safeListVarUseE_eqlLen' with t v m; 
+    try apply val_Bc; trivial.
+  - apply IHps with t v m; trivial.
+Qed.
+      
